Replace the later credits and laters in WPC with the physical step modality.

src/program_logic/crash_adequacy.v
@@ -28,153 +28,139 @@ Local Notation "'WPC' e @ s ;  E1 {{ Φ } } {{ Φc } }" := (wpc0 s mj E1 e%E Φ 
 
 Notation wptp s t := ([∗ list] ef ∈ t, WPC ef @ s; ⊤ {{ fork_post }} {{ True }})%I.
 
-Lemma wpc_step s e1 σ1 g1 ns D κ κs e2 σ2 g2 efs m Φ Φc :
+Lemma wpc_step s e1 σ1 g1 D κ κs e2 σ2 g2 efs m Φ Φc :
   prim_step e1 σ1 g1 κ e2 σ2 g2 efs →
   state_interp σ1 m -∗
-  global_state_interp g1 ns mj D (κ ++ κs) -∗
+  global_state_interp g1 mj D (κ ++ κs) -∗
   WPC e1 @ s; ⊤ {{ Φ }} {{ Φc }} -∗ NC 1 -∗
-  £ (S $ num_laters_per_step ns) -∗
-  ||={⊤|⊤,∅|∅}=> ||▷=>^(S $ num_laters_per_step ns) ||={∅|∅,⊤|⊤}=>
+  |={⊤|⊤}⧗=>
   state_interp σ2 (length efs + m) ∗
-  global_state_interp g2 (step_count_next ns) mj D κs ∗
+  global_state_interp g2 mj D κs ∗
   WPC e2 @ s; ⊤ {{ Φ }} {{ Φc }} ∗
   wptp s efs ∗
   NC 1.
 Proof.
-  rewrite {1}wpc0_unfold /wpc_pre. iIntros (?) "Hσ Hg H HNC Hlc".
+  rewrite {1}wpc0_unfold /wpc_pre. iIntros (?) "Hσ Hg H HNC".
   rewrite (val_stuck e1 σ1 g1 κ e2 σ2 g2 efs) //.
   iDestruct "H" as "(H&_)".
   iMod (fupd2_mask_subseteq ⊤ (⊤ ∖ D)) as "Hclo"; try set_solver+.
-  iMod ("H" $! _ σ1 with "Hσ Hg HNC Hlc") as "H".
-  iModIntro.
-  iApply (step_fupd2N_wand with "H"). iIntros "(_&H)".
-  iMod ("H" $! e2 σ2 g2 efs with "[//]") as "H".
-  iMod "Hclo". iModIntro. eauto.
-  destruct (to_val e2); eauto.
+  iDestruct ("H" $! _ σ1 with "Hσ Hg HNC [//]") as "H".
+  iApply (physical_step_wand with "H").
+  iIntros "(?&?&?&?)".
+  destruct (to_val e2); eauto; iFrame.
 Qed.
 
-Lemma wptp_step s e1 t1 t2 κ κs σ1 g1 ns D σ2 g2 Φ Φc :
+Lemma wptp_step s e1 t1 t2 κ κs σ1 g1 D σ2 g2 Φ Φc :
   step (e1 :: t1,(σ1,g1)) κ (t2, (σ2,g2)) →
   state_interp σ1 (length t1) -∗
-  global_state_interp g1 ns mj D (κ ++ κs) -∗
+  global_state_interp g1 mj D (κ ++ κs) -∗
   WPC e1 @ s; ⊤ {{ Φ }} {{ Φc }}-∗ wptp s t1 -∗ NC 1 -∗
-  £ (S $ num_laters_per_step ns) ==∗
   ∃ e2 t2', ⌜t2 = e2 :: t2'⌝ ∗
-  ||={⊤|⊤,∅|∅}=> ||▷=>^(S $ num_laters_per_step ns) ||={∅|∅,⊤|⊤}=>
+  |={⊤|⊤}⧗=>
   state_interp σ2 (pred (length t2)) ∗
-  global_state_interp g2 (step_count_next ns) mj D κs ∗
+  global_state_interp g2 mj D κs ∗
   WPC e2 @ s; ⊤ {{ Φ }} {{ Φc}} ∗ wptp s t2' ∗ NC 1.
 Proof.
-  iIntros (Hstep) "Hσ Hg He Ht HNC Hlc".
+  iIntros (Hstep) "Hσ Hg He Ht HNC".
   destruct Hstep as [e1' σ1' g1' e2' σ2' g2' efs [|? t1'] t2' ?? Hstep]; simplify_eq/=.
-  - iExists e2', (t2' ++ efs). iModIntro. iSplitR; first by eauto.
-    iMod (wpc_step with "Hσ Hg He HNC Hlc") as "H"; first done. iModIntro.
-    iApply (step_fupd2N_wand with "H"). iIntros ">(Hσ & Hg & He2 & Hefs) !>".
+  - iExists e2', (t2' ++ efs). iSplitR; first by eauto.
+    iDestruct (wpc_step with "Hσ Hg He HNC") as "H"; first done.
+    iApply (physical_step_wand with "H"). iIntros "(Hσ & Hg & He2 & Hefs)".
     rewrite Nat.add_comm length_app. by iFrame.
   - iExists e, (t1' ++ e2' :: t2' ++ efs); iSplitR; first eauto.
     iDestruct "Ht" as "(Ht1 & He1 & Ht2)".
-    iModIntro. iMod (wpc_step with "Hσ Hg He1 HNC Hlc") as "H"; first done. iModIntro.
-    iApply (step_fupd2N_wand with "H"). iIntros ">(Hσ & Hg & He2 & Hefs) !>".
+    iDestruct (wpc_step with "Hσ Hg He1 HNC") as "H"; first done.
+    iApply (physical_step_wand with "H"). iIntros "(Hσ & Hg & He2 & Hefs)".
     rewrite !length_app /= !length_app.
     replace (length t1' + S (length t2' + length efs))
       with (length efs + (length t1' + S (length t2'))) by lia. by iFrame.
 Qed.
-(* The total number of laters used between the physical steps number
+
+(* (* The total number of laters used between the physical steps number
    [start] (included) to [start+ns] (excluded). *)
-Local Fixpoint steps_sum (num_laters_per_step step_count_next : nat → nat) (start ns : nat) : nat :=
-  match ns with
+Local Fixpoint steps_sum (num_laters_per_step step_count_next : nat → nat) (start : nat) : nat :=
+  match with
   | O => 0
-  | S ns =>
+  | S =>
     S $ num_laters_per_step start +
     steps_sum num_laters_per_step step_count_next (step_count_next start) ns
   end.
 
-Lemma steps_sum_S (num_laters_per_step step_count_next : nat → nat) (start ns : nat) :
+Lemma steps_sum_S (num_laters_per_step step_count_next : nat → nat) (start : nat) :
   steps_sum num_laters_per_step step_count_next start (S ns) =
-  steps_sum num_laters_per_step step_count_next (step_count_next start) ns + S (num_laters_per_step start).
-Proof. induction ns => //=; try lia. Qed.
+  steps_sum num_laters_per_step step_count_next (step_count_next start) + S (num_laters_per_step start).
+Proof. induction => //=; try lia. Qed.
 
-Lemma steps_sum_S_r (num_laters_per_step step_count_next : nat → nat) (start ns : nat) :
+Lemma steps_sum_S_r (num_laters_per_step step_count_next : nat → nat) (start : nat) :
   steps_sum num_laters_per_step step_count_next start (S ns) =
-  steps_sum num_laters_per_step step_count_next start ns + S (num_laters_per_step (Nat.iter ns step_count_next start)).
+  steps_sum num_laters_per_step step_count_next start + S (num_laters_per_step (Nat.iter step_count_next start)).
 Proof.
   revert start.
-  induction ns => start.
+  induction => start.
   - rewrite //=; lia.
   - rewrite steps_sum_S IHns. simpl.
     rewrite -Nat.iter_succ_r /=. lia.
-Qed.
+Qed. *)
 
-Lemma wptp_steps s n e1 t1 κs κs' t2 σ1 g1 ns D σ2 g2 Φ Φc :
+Lemma wptp_steps s n e1 t1 κs κs' t2 σ1 g1 D σ2 g2 Φ Φc :
   nsteps n (e1 :: t1, (σ1,g1)) κs (t2, (σ2,g2)) →
   state_interp σ1 (length t1) -∗
-  global_state_interp g1 ns mj D (κs ++ κs') -∗
+  global_state_interp g1 mj D (κs ++ κs') -∗
   WPC e1 @ s; ⊤ {{ Φ }} {{ Φc }} -∗ wptp s t1 -∗ NC 1 -∗
-  £ (steps_sum num_laters_per_step step_count_next ns n) -∗
-  (||={⊤|⊤, ∅|∅}=> ||▷=>^(steps_sum num_laters_per_step step_count_next ns n) ||={∅|∅,⊤|⊤}=> ∃ e2 t2',
+  (|={⊤|⊤}⧗=>^n ∃ e2 t2',
     ⌜t2 = e2 :: t2'⌝ ∗
     state_interp σ2 (pred (length t2)) ∗
-    global_state_interp g2 (Nat.iter n step_count_next ns) mj D κs' ∗
+    global_state_interp g2 mj D κs' ∗
     WPC e2 @ s; ⊤ {{ Φ }} {{ Φc }} ∗ wptp s t2' ∗
     NC 1).
 Proof.
-  revert e1 t1 κs κs' t2 σ1 g1 ns σ2 g2; simpl.
-  induction n as [|n IH]=> e1 t1 κs κs' t2 σ1 g1 ns σ2 g2 /=.
-  { inversion_clear 1; iIntros "??????"; iExists e1, t1; iFrame; eauto 10.
-    iApply fupd2_mask_intro_subseteq; eauto. }
-  iIntros (Hsteps) "Hσ Hg He Ht HNC Hlc". inversion_clear Hsteps as [|?? [t1' [σ1' g1']]].
+  revert e1 t1 κs κs' t2 σ1 g1 σ2 g2; simpl.
+  induction n as [|n IH]=> e1 t1 κs κs' t2 σ1 g1 σ2 g2 /=.
+  { inversion_clear 1; iIntros "?????"; iExists e1, t1; iFrame; eauto 10. }
+  iIntros (Hsteps) "Hσ Hg He Ht HNC". inversion_clear Hsteps as [|?? [t1' [σ1' g1']]].
   rewrite -(assoc_L (++)).
-  rewrite -Nat.add_succ_l lc_split.
-  iDestruct "Hlc" as "[Hlc1 Hlc2]".
-  iApply step_fupd2N_inner_add.
-  iMod (wptp_step with "Hσ Hg He Ht HNC Hlc1") as (e1' t1'' ?) ">H"; first eauto; simplify_eq.
-  iApply (step_fupd2N_wand with "H"). iIntros "!> H".
-  iMod "H".
-  iDestruct "H" as "(Hσ & Hg & He & Ht & HNC)".
-  iMod (IH with "Hσ Hg He Ht HNC Hlc2") as "IH"; first done.
-  rewrite -Nat.iter_succ_r.
-  iModIntro. iModIntro. eauto.
+  iDestruct (wptp_step with "Hσ Hg He Ht HNC") as (e1' t1'' ?) "H"; first eauto; simplify_eq.
+  iApply (physical_step_wand with "H"). iIntros "(Hσ & Hg & He & Ht & HNC)".
+  by iApply (IH with "Hσ Hg He Ht HNC").
 Qed.
 
-Lemma wpc_safe κs m e σ g ns D Φ Φc q :
+Lemma wpc_safe κs m e σ g D Φ Φc q :
   state_interp σ m -∗
-  global_state_interp g ns mj D κs -∗
+  global_state_interp g mj D κs -∗
   WPC e @ ⊤ {{ Φ }} {{ Φc }} -∗ NC q -∗
-  £ (S $ num_laters_per_step ns) -∗
-  ||={⊤|⊤, ∅|∅}=> ||▷=>^(num_laters_per_step ns + 1)
+  ||={⊤|⊤, ∅|∅}=>
   ⌜is_Some (to_val e) ∨ reducible e σ g⌝.
 Proof.
   rewrite wpc0_unfold /wpc_pre. iIntros "Hσ Hg H". iDestruct "H" as "(H&_)".
   destruct (to_val e) as [v|] eqn:?.
-  { iIntros "_ _". iApply fupd2_mask_intro; [done..|].
-    iIntros "_". iApply step_fupd2N_later. auto. }
-  iIntros "HNC Hlc".
+  { iIntros "_". iApply fupd2_mask_intro; [done..|].
+    iIntros "_".  auto. }
+  iIntros "HNC".
   iMod (fupd2_mask_subseteq ⊤ (⊤ ∖ D)) as "Hclo"; try set_solver+.
-  iMod ("H" $! _ _ _ _ _ [] with "[$] [$] [$] [$]") as "H".
-  simpl. iModIntro. rewrite [_ + 1]comm. iApply (step_fupd2N_wand with "H").
-  iNext. iIntros "(%Hred&Hclo')". eauto.
+  iDestruct ("H" $! _ _ _ _ _ [] with "[$] [Hg] [$]") as "[H _]".
+  - by rewrite app_nil_r.
+  - iMod "H" as "%". iPureIntro. by right.
 Qed.
 
-Local Lemma wptp0_strong_adequacy Φ Φc κs' s n e1 t1 κs t2 σ1 g1 ns D σ2 g2 :
+Local Lemma wptp0_strong_adequacy Φ Φc κs' s n e1 t1 κs t2 σ1 g1 D σ2 g2 :
   nsteps n (e1 :: t1, (σ1,g1)) κs (t2, (σ2,g2)) →
   state_interp σ1 (length t1) -∗
-  global_state_interp g1 ns mj D (κs ++ κs') -∗
+  global_state_interp g1 mj D (κs ++ κs') -∗
   WPC e1 @ s; ⊤ {{ Φ }} {{ Φc }} -∗
   wptp s t1 -∗
   NC 1 -∗
-  £ (steps_sum num_laters_per_step step_count_next ns n) -∗
-  ||={⊤|⊤,∅|∅}=> ||▷=>^(steps_sum num_laters_per_step step_count_next ns n) ||={∅|∅, ⊤|⊤}=> (∃ e2 t2',
+  |={⊤|⊤}⧗=>^n ||={⊤|⊤,⊤|⊤}=> (∃ e2 t2',
     ⌜ t2 = e2 :: t2' ⌝ ∗
     state_interp σ2 (length t2') ∗
-    global_state_interp g2 (Nat.iter n step_count_next ns) mj D κs' ∗
+    global_state_interp g2 mj D κs' ∗
     from_option Φ True (to_val e2) ∗
     ([∗ list] v ∈ omap to_val t2', fork_post v) ∗
     NC 1).
 Proof.
-  iIntros (Hstep) "Hσ Hg He Ht HNC Hlc".
-  iMod (wptp_steps with "Hσ Hg He Ht HNC Hlc") as "Hwp"; first done.
-  iModIntro. iApply (step_fupd2N_wand with "Hwp").
-  iMod 1 as (e2' t2' ?) "(Hσ & Hg & Hwp & Ht & HNC)"; simplify_eq/=.
+  iIntros (Hstep) "Hσ Hg He Ht HNC".
+  iDestruct (wptp_steps with "Hσ Hg He Ht HNC") as "Hwp"; first done.
+  iApply (physical_stepN_wand with "Hwp").
+  iDestruct 1 as (e2' t2' ?) "(Hσ & Hg & Hwp & Ht & HNC)"; simplify_eq/=.
   iExists _, _. iSplitL ""; first done. iFrame "Hσ".
   iMod (fupd2_mask_subseteq ⊤ (⊤ ∖ D)) as "Hclo"; try set_solver+.
   iMod (wpc0_value_inv_option with "Hwp Hg HNC") as "($&Hg&HNC)".
@@ -189,62 +175,51 @@ Proof.
   + by iApply ("IH" with "[$] [$]").
 Qed.
 
-Local Lemma wptp0_progress Φ Φc κs' n e1 t1 κs t2 σ1 g1 ns D σ2 g2 e2 :
+Local Lemma wptp0_progress Φ Φc κs' n e1 t1 κs t2 σ1 g1 D σ2 g2 e2 :
   nsteps n (e1 :: t1, (σ1,g1)) κs (t2, (σ2,g2)) →
   e2 ∈ t2 →
   state_interp σ1 (length t1) -∗
-  global_state_interp g1 ns mj D (κs ++ κs') -∗
+  global_state_interp g1 mj D (κs ++ κs') -∗
   WPC e1 @ NotStuck; ⊤ {{ Φ }} {{ Φc }} -∗
   wptp NotStuck t1 -∗
   NC 1 -∗
-  £ (steps_sum num_laters_per_step step_count_next ns (S n)) -∗
-  ||={⊤|⊤,∅|∅}=> ||▷=>^(steps_sum num_laters_per_step step_count_next ns n) ||={∅|∅, ∅|∅}=>
-  ||▷=>^(num_laters_per_step (Nat.iter n step_count_next ns) + 1)
+  |={⊤|⊤}⧗=>^n ||={⊤|⊤, ∅|∅}=>
    ⌜ not_stuck e2 σ2 g2 ⌝.
 Proof.
-  iIntros (Hstep Hel) "Hσ Hg He Ht HNC Hlc".
+  iIntros (Hstep Hel) "Hσ Hg He Ht HNC".
   rewrite steps_sum_S_r.
-  iDestruct "Hlc" as "[Hlc1 Hlc2]".
-  iMod (wptp_steps with "Hσ Hg He Ht HNC Hlc1") as "Hwp"; first done.
-  iModIntro. iApply (step_fupd2N_wand with "Hwp").
+  iMod (wptp_steps with "Hσ Hg He Ht HNC") as "Hwp"; first done.
+  iModIntro. iApply (physical_stepN_wand with "Hwp").
   iMod 1 as (e2' t2' ?) "(Hσ & Hg & Hwp & Ht & HNC)"; simplify_eq/=.
   apply elem_of_cons in Hel as [<-|(t1''&t2''&->)%elem_of_list_split].
-  - iPoseProof (wpc_safe with "Hσ Hg Hwp HNC Hlc2") as "H".
+  - iPoseProof (wpc_safe with "Hσ Hg Hwp HNC") as "H".
     iMod "H". eauto.
   - iDestruct "Ht" as "(_ & He' & _)".
-    iPoseProof (wpc_safe with "Hσ Hg He' HNC Hlc2") as "H".
+    iPoseProof (wpc_safe with "Hσ Hg He' HNC") as "H".
     by iMod "H".
 Qed.
 
-Local Lemma wptp0_strong_crash_adequacy Φ Φc κs' s n e1 t1 κs t2 σ1 g1 ns D σ2 g2 :
+Local Lemma wptp0_strong_crash_adequacy Φ Φc κs' s n e1 t1 κs t2 σ1 g1 D σ2 g2 :
   nsteps n (e1 :: t1, (σ1, g1)) κs (t2, (σ2, g2)) →
   state_interp σ1 (length t1) -∗
-  global_state_interp g1 ns mj D (κs ++ κs') -∗
+  global_state_interp g1 mj D (κs ++ κs') -∗
   WPC e1 @ s; ⊤ {{ Φ }} {{ Φc }} -∗
   wptp s t1 -∗
   NC 1 -∗
-  £ (steps_sum num_laters_per_step step_count_next ns (S n)) -∗
-  ||={⊤|⊤,∅|∅}=> ||▷=>^(steps_sum num_laters_per_step step_count_next ns (S n)) ||={∅|∅, ⊤|⊤}=>
-  ▷ (∃ e2 t2',
+  |={⊤|⊤}⧗=>^n ||={⊤|⊤,⊤|⊤}=>
+  (∃ e2 t2',
     ⌜ t2 = e2 :: t2' ⌝ ∗
-    Φc ∗ state_interp σ2 (length t2') ∗ global_state_interp g2 ((Nat.iter n step_count_next ns)) mj D κs' ∗ C).
+    Φc ∗ state_interp σ2 (length t2') ∗ global_state_interp g2 mj D κs' ∗ C).
 Proof.
-  iIntros (Hstep) "Hσ Hg He Ht HNC Hlc".
-  rewrite steps_sum_S_r.
-  iDestruct "Hlc" as "[Hlc1 Hlc2]".
-  iDestruct (wptp_steps with "Hσ Hg He Ht HNC Hlc1") as "Hwp"; first done.
-  iApply step_fupd2N_inner_add.
-  iApply (step_fupd2N_inner_wand with "Hwp"); auto.
+  iIntros (Hstep) "Hσ Hg He Ht HNC".
+  iDestruct (wptp_steps with "Hσ Hg He Ht HNC") as "Hwp"; first done.
+  iApply (physical_stepN_wand with "[$]").
   iDestruct 1 as (e2' t2' ?) "(Hσ & Hg & Hwp & Ht & HNC)"; simplify_eq/=.
   iMod (fupd2_mask_subseteq ⊤ (⊤ ∖ D)) as "Hclo"; try set_solver+.
   iMod (NC_upd_C with "HNC") as "#HC".
-  iPoseProof (wpc0_crash with "[$] Hg [$]") as "H".
-  iMod "Hclo".
-  iDestruct "Hlc2" as "[_ Hlc2]".
-  iSpecialize ("H" with "[$]").
-  iApply (step_fupd2N_inner_wand _ _ _ _ (S _) with "H"); auto.
-  iIntros "(Hg&HΦc)". iNext. iExists _, _. iSplitL ""; first done.
-  iFrame. eauto.
+  iPoseProof (wpc0_crash with "[$] Hg [$]") as ">[$$]".
+  iMod "Hclo". iFrame "#∗".
+  iModIntro. by iExists _.
 Qed.
 End crash_adequacy.
 
@@ -260,66 +235,62 @@ Implicit Types Φs : list (val Λ → iProp Σ).
 
 Notation wptp s t := ([∗ list] ef ∈ t, WPC ef @ s; ⊤ {{ fork_post }} {{ True }})%I.
 
-Lemma wptp_strong_adequacy Φ Φc κs' s n e1 t1 κs t2 σ1 g1 ns mj D σ2 g2 :
+Lemma wptp_strong_adequacy Φ Φc κs' s n e1 t1 κs t2 σ1 g1 mj D σ2 g2 :
   nsteps n (e1 :: t1, (σ1, g1)) κs (t2, (σ2, g2)) →
   state_interp σ1 (length t1) -∗
-  global_state_interp g1 ns mj D (κs ++ κs') -∗
+  global_state_interp g1 mj D (κs ++ κs') -∗
   WPC e1 @ s; ⊤ {{ Φ }} {{ Φc }} -∗
   wptp s t1 -∗
   NC 1 -∗
-  £ (steps_sum num_laters_per_step step_count_next ns n) -∗
-  ||={⊤|⊤,∅|∅}=> ||▷=>^(steps_sum num_laters_per_step step_count_next ns n) ||={∅|∅, ⊤|⊤}=> (∃ e2 t2',
+  |={⊤|⊤}⧗=>^n ||={⊤|⊤,⊤|⊤}=> (∃ e2 t2',
     ⌜ t2 = e2 :: t2' ⌝ ∗
     state_interp σ2 (length t2') ∗
-    global_state_interp g2 ((Nat.iter n step_count_next ns)) mj D κs' ∗
+    global_state_interp g2 mj D κs' ∗
     from_option Φ True (to_val e2) ∗
     ([∗ list] v ∈ omap to_val t2', fork_post v) ∗
     NC 1).
 Proof.
-  iIntros (?) "?? Hwpc Hwptp Hnc Hlc".
-  iApply (wptp0_strong_adequacy mj with "[$] [$] [Hwpc] [Hwptp] [$] [$]"); first eassumption.
+  iIntros (?) "?? Hwpc Hwptp Hnc".
+  iApply (wptp0_strong_adequacy mj with "[$] [$] [Hwpc] [Hwptp] [$]"); first eassumption.
   { by iApply wpc0_wpc. }
   { iApply (big_sepL_mono with "Hwptp"). iIntros.
     iApply (wpc0_wpc); eauto.
   }
 Qed.
 
-Lemma wptp_progress Φ Φc κs' n e1 t1 κs t2 σ1 g1 ns mj D σ2 g2 e2 :
+Lemma wptp_progress Φ Φc κs' n e1 t1 κs t2 σ1 g1 mj D σ2 g2 e2 :
   nsteps n (e1 :: t1, (σ1, g1)) κs (t2, (σ2, g2)) →
   e2 ∈ t2 →
   state_interp σ1 (length t1) -∗
-  global_state_interp g1 ns mj D (κs ++ κs') -∗
+  global_state_interp g1 mj D (κs ++ κs') -∗
   WPC e1 @ NotStuck; ⊤ {{ Φ }} {{ Φc }} -∗
   wptp NotStuck t1 -∗
   NC 1 -∗
-  £ (steps_sum num_laters_per_step step_count_next ns (S n)) -∗
-  ||={⊤|⊤,∅|∅}=> ||▷=>^(steps_sum num_laters_per_step step_count_next ns n) ||={∅|∅, ∅|∅}=>
-  ||▷=>^(num_laters_per_step (Nat.iter n step_count_next ns) + 1)
+  |={⊤|⊤}⧗=>^n ||={⊤|⊤,∅|∅}=>
   (⌜not_stuck e2 σ2 g2 ⌝).
 Proof.
-  iIntros (??) "?? Hwpc Hwptp Hnc Hlc".
-  iApply (wptp0_progress mj with "[$] [$] [Hwpc] [Hwptp] [$] [$]"); first done; first done.
+  iIntros (??) "?? Hwpc Hwptp Hnc".
+  iApply (wptp0_progress mj with "[$] [$] [Hwpc] [Hwptp] [$]"); first done; first done.
   { by iApply wpc0_wpc. }
   { iApply (big_sepL_mono with "Hwptp"). iIntros.
     iApply (wpc0_wpc); eauto.
   }
 Qed.
 
-Lemma wptp_strong_crash_adequacy Φ Φc κs' s n e1 t1 κs t2 σ1 g1 ns mj D σ2 g2 :
+Lemma wptp_strong_crash_adequacy Φ Φc κs' s n e1 t1 κs t2 σ1 g1 mj D σ2 g2 :
   nsteps n (e1 :: t1, (σ1, g1)) κs (t2, (σ2, g2)) →
   state_interp σ1 (length t1) -∗
-  global_state_interp g1 ns mj D (κs ++ κs') -∗
+  global_state_interp g1 mj D (κs ++ κs') -∗
   WPC e1 @ s; ⊤ {{ Φ }} {{ Φc }} -∗
   wptp s t1 -∗
   NC 1 -∗
-  £ (steps_sum num_laters_per_step step_count_next ns (S n)) -∗
-  ||={⊤|⊤,∅|∅}=> ||▷=>^(steps_sum num_laters_per_step step_count_next ns (S n)) ||={∅|∅, ⊤|⊤}=>
-  ▷ (∃ e2 t2',
+  |={⊤|⊤}⧗=>^n ||={⊤|⊤,⊤|⊤}=>
+  (∃ e2 t2',
     ⌜ t2 = e2 :: t2' ⌝ ∗
-    Φc ∗ state_interp σ2 (length t2') ∗ global_state_interp g2 (Nat.iter n step_count_next ns) mj D κs' ∗ C).
+    Φc ∗ state_interp σ2 (length t2') ∗ global_state_interp g2 mj D κs' ∗ C).
 Proof.
-  iIntros (?) "?? Hwpc Hwptp Hnc Hlc".
-  iApply (wptp0_strong_crash_adequacy mj with "[$] [$] [Hwpc] [Hwptp] [$] Hlc"); first eassumption.
+  iIntros (?) "?? Hwpc Hwptp Hnc".
+  iApply (wptp0_strong_crash_adequacy mj with "[$] [$] [Hwpc] [Hwptp] [$]"); first eassumption.
   { by iApply wpc0_wpc. }
   { iApply (big_sepL_mono with "Hwptp"). iIntros.
     iApply (wpc0_wpc); eauto.
