flake.nix
@@ -11,39 +11,78 @@
     nix-vscode-extensions.url = "github:nix-community/nix-vscode-extensions";
   };
 
-  outputs = {
-    nixpkgs,
-    flake-utils,
-    grackle,
-    ...
-  }:
-    flake-utils.lib.eachDefaultSystem (
-      system: let
-        pkgs = import nixpkgs {
-          inherit system;
+  outputs = {nixpkgs, ...}@inputs: let
+    system = "x86_64-linux";
+    codium_settings = ./codium-settings.json;
+  in {
+    devShells."${system}".default = let
+      pkgs = import nixpkgs {
+        inherit system;
+        config.allowUnfree = true;
+      };
+      opam-nix = inputs.opam-nix.lib.${system};
+      grackle = pkgs.buildGoModule {
+        name = "grackle";
+        src = pkgs.fetchFromGitHub {
+          owner = "mjschwenne";
+          repo = "grackle";
+          rev = "3a83c3b22f163da77d75bfdb3923f007af2ad515";
+          sha256 = "1bl8lx50qhl6yczjnwfwywx29nvinr20v2zjdc2zjqi8kcls7kqr";
         };
-      in {
-        devShells.default = with pkgs;
-          mkShell {
-            buildInputs = [
-              coq
-              coqPackages.stdlib
+        vendorHash = "sha256-c9+npmcdynfqSnxEZSdubVeN8Y3eYAwjya52vTJayY0=";
+        checkPhase = false;
+      };
+      goose = pkgs.buildGoModule {
+        name = "goose";
+        src = pkgs.fetchFromGitHub {
+          owner = "goose-lang";
+          repo = "goose";
+          rev = "67cf95ebfc80e80ddc40b0518e6d761cde44977c";
+          sha256 = "16040c4frxn9dk3xmajzg4jb7fi7q39hasfp94rpnphmpr4hvr51";
+        };
+        vendorHash = "sha256-HCJ8v3TSv4UrkOsRuENWVz5Z7zQ1UsOygx0Mo7MELzY=";
+      };
+      repos = [ "${inputs.opam-repository}" "${inputs.opam-coq-repository}" ];
+      scope = opam-nix.queryToScope { inherit repos; } ({ ocaml-base-compiler = "*"; "coq" = "8.20.1"; vscoq-language-server = "*"; });
 
-              go
-              grackle.packages.${system}.default
-              grackle.packages.${system}.goose
-              protobuf
+      vscode-marketplace = inputs.nix-vscode-extensions.extensions.${system}.vscode-marketplace;
+      vscode-marketplace-correct = inputs.nix-vscode-extensions.extensions.${system}.forVSCodeVersion "1.100.0";
+      vscode = import /research/nix/vscode-no-state.nix {
+        inherit pkgs vscode-marketplace;
 
-              # nix helpers
-              nix-prefetch-git
-              nix-prefetch-github
-              nix-prefetch
-            ];
+        settings = codium_settings;
+        vscodeExtensions = with vscode-marketplace; [
+          maximedenes.vscoq
+          leanprover.lean4
+        ];
+      };
+      
+    in
+      pkgs.mkShell {
+        packages = [
+          # coq deps
+          scope.coq
+          scope.vscoq-language-server
+
+          vscode
+
+          pkgs.python3
+
+          pkgs.go
+          grackle
+          goose
+          pkgs.protobuf
+
+          # nix helper
+          # Should be able to update goose and grackle with `update-nix-fetchgit flake.nix`
+          pkgs.update-nix-fetchgit
+          pkgs.nix-prefetch-git
+          pkgs.nix-prefetch
+        ];
 
             shellHook = ''
               unset COQPATH
             '';
           };
-      }
-    );
+      };
 }
